# baseURI: http://crowddata.abdn.ac.uk/ontologies/ka/form-requirements
# imports: http://rdfs.org/ns/void

@prefix form-requirements: <http://crowddata.abdn.ac.uk/ontologies/ka/form-requirements#> .
@prefix owl: <http://www.w3.org/2002/07/owl#> .
@prefix rdf: <http://www.w3.org/1999/02/22-rdf-syntax-ns#> .
@prefix rdfs: <http://www.w3.org/2000/01/rdf-schema#> .
@prefix xsd: <http://www.w3.org/2001/XMLSchema#> .
@prefix cd: <http://crowddata.abdn.ac.uk/ontologies/cd/0.1/> .




<http://crowddata.abdn.ac.uk/ontologies/ka/form-requirements>
  rdf:type owl:Ontology ;
  owl:imports <http://rdfs.org/ns/void> ;
  owl:versionInfo "Created with TopBraid Composer"^^xsd:string ;
.


cd:sparqlQuery a owl:DatatypeProperty;
rdfs:domain form-requirements:PropertyDescription;
rdfs:range xsd:string;
rdfs:label "Sparql Query";
rdfs:comment "Sparql SELECT Query to retrieve value and label instances for a particular property" .

cd:sparqlEndpoint a owl:ObjectProperty;
rdfs:domain form-requirements:PropertyDescription;
rdfs:range rdfs:Resource;
rdfs:label "Sparql Endpoint";
rdfs:comment "Endpoint for SPARQL query to be executed from" .


form-requirements:PropertyDescription
rdfs:label "Property Description" ;
rdfs:comment "Additional property descriptions for RDForm template generation";
  rdf:type rdfs:Class ;
  rdfs:subClassOf [
      rdf:type owl:Restriction ;
      owl:cardinality "1"^^xsd:nonNegativeInteger ;
      owl:onProperty rdfs:label ;
    ] ;
  rdfs:subClassOf [
      rdf:type owl:Restriction ;
      owl:maxCardinality "1"^^xsd:nonNegativeInteger ;
      owl:onProperty rdfs:comment ;
    ] ;
	
.
form-requirements:dataset
  rdf:type owl:ObjectProperty ;
  rdfs:range rdfs:Resource ;
.

form-requirements:ClassDescription
rdfs:label "Class Description" ;
rdfs:comment "Additional class descriptions for RDForm template generation";
.

form-requirements:dataset
  rdf:type owl:ObjectProperty ;
  rdfs:range rdfs:Resource ;
.